Pure.Basic

Iterator/Pure/Basic.lean
@@ -8,3 +8,81 @@ def Iter.toIterM {α : Type w} {β : Type v} (it : Iter (α := α) β) : IterM (
 
 def IterM.toPureIter {α : Type w} {β : Type v} (it : IterM (α := α) Id β) : Iter (α := α) β :=
   ⟨it.inner⟩
+
+@[simp]
+theorem Iter.toPureIter_toIterM {α : Type w} {β : Type v} (it : Iter (α := α) β) :
+    it.toIterM.toPureIter = it :=
+  rfl
+
+@[simp]
+theorem Iter.toIterM_toPureIter {α : Type w} {β : Type v} (it : IterM (α := α) Id β) :
+    it.toPureIter.toIterM = it :=
+  rfl
+
+def Iter.plausible_step {α : Type w} {β : Type v} [Iterator α Id β]
+    (it : Iter (α := α) β) (step : IterStep (Iter (α := α) β) β) : Prop :=
+  it.toIterM.plausible_step (step.map Iter.toIterM id)
+
+def Iter.Step {α : Type w} {β : Type v} [Iterator α Id β] (it : Iter (α := α) β) :=
+  PlausibleIterStep (Iter.plausible_step it)
+
+def Iter.plausible_output {α : Type w} {β : Type v} [Iterator α Id β]
+    (it : Iter (α := α) β) (out : β) : Prop :=
+  ∃ it', it.plausible_step (.yield it' out)
+
+def Iter.plausible_successor_of {α : Type w} {β : Type v} [Iterator α Id β]
+    (it' it : Iter (α := α) β) : Prop :=
+  ∃ step, step.successor = some it' ∧ it.plausible_step step
+
+def Iter.plausible_skip_successor_of {α : Type w} {β : Type v} [Iterator α Id β]
+    (it' it : Iter (α := α) β) : Prop :=
+  it.plausible_step (.skip it')
+
+@[always_inline, inline]
+def Iter.step {α : Type w} {β : Type w} [Iterator α Id β] [Functor Id]
+    (it : Iter (α := α) β) : it.Step := by
+  refine it.toIterM.stepH.run.inflate.map IterM.toPureIter id _ ?_
+  intro step hp
+  simp only [Iter.plausible_step, IterStep.map_map, id_eq, IterStep.map_id', toIterM_toPureIter, hp]
+
+section Finite
+
+def Iter.finitelyManySteps {α : Type w} {β : Type v} [Iterator α Id β] [Finite α Id]
+    (it : Iter (α := α) β) : IterM.TerminationMeasures.Finite α Id :=
+  it.toIterM.finitelyManySteps
+
+theorem Iter.TerminationMeasures.Finite.rel_of_yield
+    {α : Type w} {β : Type v} [Iterator α Id β]
+    {it it' : Iter (α := α) β} {out : β} (h : it.plausible_step (.yield it' out)) :
+    IterM.TerminationMeasures.Finite.rel ⟨it'.toIterM⟩ ⟨it.toIterM⟩ :=
+  IterM.TerminationMeasures.Finite.rel_of_yield h
+
+theorem Iter.TerminationMeasures.Finite.rel_of_skip
+    {α : Type w} {β : Type v} [Iterator α Id β]
+    {it it' : Iter (α := α) β} (h : it.plausible_step (.skip it')) :
+    IterM.TerminationMeasures.Finite.rel ⟨it'.toIterM⟩ ⟨it.toIterM⟩ :=
+  IterM.TerminationMeasures.Finite.rel_of_skip h
+
+macro_rules | `(tactic| decreasing_trivial) => `(tactic|
+  first
+  | exact Iter.TerminationMeasures.Finite.rel_of_yield ‹_›
+  | exact Iter.TerminationMeasures.Finite.rel_of_skip ‹_›)
+
+end Finite
+
+section Productive
+
+def Iter.finitelyManySkips {α : Type w} {β : Type v} [Iterator α Id β] [Productive α Id]
+    (it : Iter (α := α) β) : IterM.TerminationMeasures.Productive α Id :=
+  it.toIterM.finitelyManySkips
+
+theorem Iter.TerminationMeasures.Productive.rel_of_skip
+    {α : Type w} {β : Type v} [Iterator α Id β]
+    {it it' : Iter (α := α) β} (h : it.plausible_step (.skip it')) :
+    IterM.TerminationMeasures.Productive.rel ⟨it'.toIterM⟩ ⟨it.toIterM⟩ :=
+  IterM.TerminationMeasures.Productive.rel_of_skip h
+
+macro_rules | `(tactic| decreasing_trivial) => `(tactic|
+  exact Iter.TerminationMeasures.Productive.rel_of_skip ‹_›)
+
+end Productive
